\begin{samepage}
\def\no{19}
% \def\aroundarrows{\mspace{18mu}}
% \def\andsoarrow{\Rightarrow}
\begin{align*}
% \renewcommand{\baselinestretch}{2}
{I}_{\no}
=&  \int{ \frac{ 1 }{ a^2-u^2 } }\dif{u} \\
=&  \int{ \frac{ A }{ a+u } + \frac{ B }{ a-u } }\dif{u}
\nb{\sub*{}}[\quad
  A(a-u)+B(a+u) = 1
  \andso A+B=\tfrac{1}{a} \quad \text{and}\quad  B-A=0 \\
  \andso B=A
  \andso 2A=\tfrac{1}{a}
  \andso A=\tfrac{1}{2a}
  \andso B=\tfrac{1}{2a}
]
=&  \int \frac{ \frac{1}{2a} }{ a+u }
        + \frac{ \frac{-1}{2a} }{ a-u }
    \dif{u} \\
%
=&  \frac{1}{2a} \cdot \int
       \frac{ 1 }{ a+u } + \frac{ 1 }{ a-u }
    \dif{u}
%
\nb{Rearranging so \(u\) preceeds \(a\) for aesthetic reasons}
%
=&  \frac{1}{2a} \cdot \int
       \frac{ 1 }{ u+a } - \frac{ 1 }{ u-a }
    \dif{u} \\
%
=&  \frac{1}{2a} \left(
      \ln\abs{ u+a } - \ln\abs{ u-a }
    \right) +C \\
%
=&  \frac{1}{2a} \cdot { \ln\abs{ \frac{u+a}{ u-a } } }+C
\end{align*}


\footeqn{\no}{
%
\int{\frac{ 1 }{ a^2-u^2 } \dif{u}}%
=\frac{1}{2a} { \ln\abs{ \frac{u+a}{u-a} } }+C
%
}

\end{samepage}
