\begingroup
\begin{center}
\textbf{Important Maclaurin Series}
\end{center}
\[
\setlength\jot{3em}
\begin{alignedat}{3}
\frac{1}{1-x}
\;&=\;    \sum_{n=0}^\infty  x^n
&\;&=\;   1 + x + x^2 + x^3 + \cdots
\quad&R&=1
\\
e^x
\;&=\;
\sum_{n=0}^\infty\frac{x^n}{n!}
&\;&=\;
1 + \frac{x}{1!}+\frac{x^2}{2!}+\frac{x^3}{3!}+\cdots
\quad&R&=\infty
\\
\sin x
\;&=\;
\sum_{n=0}^\infty{(-1)}^{n}\frac{x^{2n+1}}{(2n+1)!}
&\;&=\;
x - \frac{x^3}{3!}+\frac{x^5}{5!}-\frac{x^7}{7!}+\cdots
\quad&R&=\infty
\\
\cos x
\;&=\;
\sum_{n=0}^\infty  {(-1)}^{n} \frac{ x^{2n} }{ (2n)! }
&\;&=\;
1 - \frac{x^2}{2!}+\frac{x^4}{4!}-\frac{x^6}{6!}+\cdots
\quad&R&=\infty
\\
\tan^{-1} x
\;&=\;    \sum_{n=0}^\infty  {(-1)}^{n} \frac{ x^{2n+1} }{ 2n+1 }
&\;&=\;   x - \frac{x^3}{3} + \frac{x^5}{5} - \frac{x^7}{7} + \cdots
\quad&R&=1
\\
\ln(1+x)
\;&=\;    \sum_{n=1}^\infty  {(-1)}^{n-1} \frac{ x^{n} }{ n }
&\;&=\;   x - \frac{x^2}{2} + \frac{x^3}{3} - \frac{x^4}{4} + \cdots
\quad&R&=1
\\
{(1+x)}^k
\;&=\;   \sum_{n=0}^\infty  \binom{k}{n}x^n
&\;&
\begin{multlined}[t]
=\;  1 + kx + \frac{k(k-1)}{2!}x^2 \\[-2em]
                            + \frac{k(k-1)(k-2)}{3!}x^3 \cdots
\end{multlined}
\quad&R&=1
\\
\end{alignedat}
\]

\endgroup
